SP1Operations/OrOperation.lean
@@ -1,0 +1,57 @@
+import SP1Foundations
+
+/-- OrOperation is only operating on `U8` because it's used solely for
+computing the or operation over four **bytes**. -/
+structure OrOperation where
+  value : Vector U8 WORD_BYTE_SIZE
+
+namespace OrOperation
+
+/-- `OrOperation` should result in and of all 4 limbs -/
+def spec (cols : OrOperation)
+    (a b : Vector (BabyBear) WORD_BYTE_SIZE)
+    (is_real : BabyBear) : Prop :=
+  is_real ≠ 0 → ∀ i : Fin WORD_BYTE_SIZE,
+    a[i] ||| b[i] = cols.value[i]
+
+/-- Constraints on `OrOperation` as extracted from the source code:
+Sends: AirInteraction { values: [1, cols.value[0], a[0], b[0]], multiplicity: is_real, kind: Byte }
+Sends: AirInteraction { values: [1, cols.value[1], a[1], b[1]], multiplicity: is_real, kind: Byte }
+Sends: AirInteraction { values: [1, cols.value[2], a[2], b[2]], multiplicity: is_real, kind: Byte }
+Sends: AirInteraction { values: [1, cols.value[3], a[3], b[3]], multiplicity: is_real, kind: Byte } -/
+def extractedConstraints (cols : OrOperation)
+    (a b : Vector (BabyBear) WORD_BYTE_SIZE) (is_real : BabyBear) :
+    List (SP1Constraint) :=
+  [
+  .sendAirInteraction_byte (.ofNat 1) cols.value[0] a[0] b[0] is_real,
+  .sendAirInteraction_byte (.ofNat 1) cols.value[1] a[1] b[1] is_real,
+  .sendAirInteraction_byte (.ofNat 1) cols.value[2] a[2] b[2] is_real,
+  .sendAirInteraction_byte (.ofNat 1) cols.value[3] a[3] b[3] is_real,
+  ]
+
+/-- Cleaned up representation of the `OrOperation` constraints. -/
+def idealizedConstraints (cols : OrOperation)
+    (a b : Vector (BabyBear) WORD_BYTE_SIZE) : Prop :=
+  a[0] ||| b[0] = cols.value[0] ∧
+  a[1] ||| b[1] = cols.value[1] ∧
+  a[2] ||| b[2] = cols.value[2] ∧
+  a[3] ||| b[3] = cols.value[3]
+
+/-- The idealized constraints are logically equivalent to the extracted ones when `is_real := 1` -/
+lemma extractedConstraints_iff_idealizedConstraints
+    (cols : OrOperation) (a b : Vector (BabyBear) WORD_BYTE_SIZE) :
+    constraintList_toProp (cols.extractedConstraints a b 1) ↔
+      cols.idealizedConstraints a b := by
+  simp [extractedConstraints, idealizedConstraints]
+  tauto
+
+/-- The extracted constraints on `OrOperation` imply the spec. -/
+theorem correct (cols : OrOperation)
+    (a b : Vector (BabyBear) WORD_BYTE_SIZE) (is_real : BabyBear) :
+    cols.idealizedConstraints a b → cols.spec a b is_real := by
+  simp [idealizedConstraints, spec, sub_eq_zero, mul_eq_zero]
+  intros h1 h2 h3 h4 hreal i
+  match i with | 0 => ?_ | 1 => ?_ | 2 => ?_ | 3 => ?_
+  all_goals trivial
+
+end OrOperation
